@prefix : <https://w3id.org/tido#> .
@prefix owl: <http://www.w3.org/2002/07/owl#> .
@prefix rdf: <http://www.w3.org/1999/02/22-rdf-syntax-ns#> .
@prefix xml: <http://www.w3.org/XML/1998/namespace> .
@prefix xsd: <http://www.w3.org/2001/XMLSchema#> .
@prefix rdfs: <http://www.w3.org/2000/01/rdf-schema#> .
@base <https://w3id.org/tido#> .

<https://w3id.org/tido> rdf:type owl:Ontology ;
                         owl:versionIRI <https://w3id.org/tido/1.0.0> ;
                         <http://purl.org/dc/terms/created> "2025-05-07"^^xsd:date ;
                         <http://purl.org/dc/terms/description> "The TIDO ontology can be used to describe the decision processes within the threat intelligence domain"@en ;
                         <http://purl.org/dc/terms/license> <https://creativecommons.org/licenses/by/4.0/> ;
                         <http://purl.org/dc/terms/title> "The Threat Intelligence Decision Ontology"@en ;
                         <http://purl.org/vocab/vann/preferredNamespacePrefix> "tido" ;
                         <http://purl.org/vocab/vann/preferredNamespaceUri> : ;
                         owl:versionInfo "1.0.0" ;
                         <https://w3id.org/mod#createdWith> <https://chowlk.linkeddata.es/> .

#################################################################
#    Annotation properties
#################################################################

###  http://purl.org/dc/terms/created
<http://purl.org/dc/terms/created> rdf:type owl:AnnotationProperty .


###  http://purl.org/dc/terms/description
<http://purl.org/dc/terms/description> rdf:type owl:AnnotationProperty .


###  http://purl.org/dc/terms/license
<http://purl.org/dc/terms/license> rdf:type owl:AnnotationProperty .


###  http://purl.org/dc/terms/title
<http://purl.org/dc/terms/title> rdf:type owl:AnnotationProperty .


###  http://purl.org/vocab/vann/preferredNamespacePrefix
<http://purl.org/vocab/vann/preferredNamespacePrefix> rdf:type owl:AnnotationProperty .


###  http://purl.org/vocab/vann/preferredNamespaceUri
<http://purl.org/vocab/vann/preferredNamespaceUri> rdf:type owl:AnnotationProperty .


###  http://www.w3.org/2002/07/owl#versionIRI
owl:versionIRI rdf:type owl:AnnotationProperty .


###  http://www.w3.org/2002/07/owl#versionInfo
owl:versionInfo rdf:type owl:AnnotationProperty .


###  http://www.w3.org/2004/02/skos/core#altLabel
<http://www.w3.org/2004/02/skos/core#altLabel> rdf:type owl:AnnotationProperty .


###  https://w3id.org/mod#createdWith
<https://w3id.org/mod#createdWith> rdf:type owl:AnnotationProperty .


#################################################################
#    Datatypes
#################################################################

###  http://www.w3.org/2001/XMLSchema#date
xsd:date rdf:type rdfs:Datatype .


#################################################################
#    Object Properties
#################################################################

###  http://www.w3.org/ns/prov#wasGeneratedBy
<http://www.w3.org/ns/prov#wasGeneratedBy> rdf:type owl:ObjectProperty ;
                                           rdfs:label "was generated by" .


###  http://www.w3.org/ns/prov#wasMemberOf
<http://www.w3.org/ns/prov#wasMemberOf> rdf:type owl:ObjectProperty ;
                                        rdfs:label "was member of" .


###  https://w3id.org/tido#answers
:answers rdf:type owl:ObjectProperty ;
         rdfs:domain :PieceOfInformation ;
         rdfs:range :RQ ;
         rdfs:comment "A piece of information can be used to answer a research question. This piece of information can be anything, as long as it can be expressed in a sentence" ;
         rdfs:label "answers" .


###  https://w3id.org/tido#assumes
:assumes rdf:type owl:ObjectProperty ;
         rdfs:domain :Option ;
         rdfs:range :Hypothesis ;
         rdfs:comment "A relationship indicating how an option would take an hypothesis as granted or true" ;
         rdfs:label "assumes" ;
         rdfs:seeAlso "https://www.merriam-webster.com/dictionary/assume" .


###  https://w3id.org/tido#contributesTo
:contributesTo rdf:type owl:ObjectProperty ;
               rdfs:domain :Activity ;
               rdfs:range :Case ;
               rdfs:comment "Every activity should contribute to one or more cases/investigations. " ;
               rdfs:label "contributes to" .


###  https://w3id.org/tido#disputes
:disputes rdf:type owl:ObjectProperty ;
          rdfs:subPropertyOf :providesInsightsInto ;
          rdfs:domain :PieceOfInformation ;
          rdfs:range :Hypothesis ;
          rdfs:comment "A relationship indicating how a piece of information calls into question or casts doubt upon a hypothesis" ;
          rdfs:label "disputes" ;
          rdfs:seeAlso "https://www.merriam-webster.com/dictionary/dispute" .


###  https://w3id.org/tido#hasConsideration
:hasConsideration rdf:type owl:ObjectProperty ;
                  rdfs:domain :Option ;
                  rdfs:range :Consideration ;
                  rdfs:comment "An option can have multiple considerations that help in deciding on whether on not to select that option" ;
                  rdfs:label "has consideration" .


###  https://w3id.org/tido#hasContext
:hasContext rdf:type owl:ObjectProperty ;
            rdfs:domain :PieceOfInformation ;
            rdfs:range :PieceOfInformation ;
            rdfs:comment "A relationship indicating how one piece of information provides relevant context to another piece of information." ;
            rdfs:label "has context" .


###  https://w3id.org/tido#informs
:informs rdf:type owl:ObjectProperty ;
         rdfs:domain :Option ;
         rdfs:range :RQ ;
         rdfs:comment "A relationship that indicates which options would aid answering a research question. " ;
         rdfs:label "informs" .


###  https://w3id.org/tido#investigates
:investigates rdf:type owl:ObjectProperty ;
              rdfs:domain :Case ;
              rdfs:range :RQ ;
              rdfs:comment "An investigation, or case, investigates one or more research questions" ;
              rdfs:label "investigates" .


###  https://w3id.org/tido#providesInsightsInto
:providesInsightsInto rdf:type owl:ObjectProperty ;
                      rdfs:domain :PieceOfInformation ;
                      rdfs:range :Hypothesis ;
                      rdfs:comment "The super-property of tido:supports and tido:disputes" ;
                      rdfs:label "provides insights into" ;
                      <http://www.w3.org/2004/02/skos/core#altLabel> "provides insight into" .


###  https://w3id.org/tido#questions
:questions rdf:type owl:ObjectProperty ;
           rdfs:domain :RQ ;
           rdfs:range :PieceOfInformation ;
           rdfs:comment "A research question can be raised by a piece of information" ;
           rdfs:label "questions" .


###  https://w3id.org/tido#supports
:supports rdf:type owl:ObjectProperty ;
          rdfs:subPropertyOf :providesInsightsInto ;
          rdfs:domain :PieceOfInformation ;
          rdfs:range :Hypothesis ;
          rdfs:comment "A relationship indicating how a piece of information provides a hypothesis with substantiation/to support with evidence or authority, making it more certain" ;
          rdfs:label "supports" ;
          rdfs:seeAlso "https://www.merriam-webster.com/dictionary/supports and https://www.merriam-webster.com/dictionary/corroborate" .


###  https://w3id.org/tido#wasExecutedBy
:wasExecutedBy rdf:type owl:ObjectProperty ;
               rdfs:domain :Option ;
               rdfs:range :Activity ;
               rdfs:comment "Once an option is selected, it could be excecuted by an activity. " ;
               rdfs:label "was executed by" .


###  https://w3id.org/tido#wasRecalledBy
:wasRecalledBy rdf:type owl:ObjectProperty ;
               rdfs:domain :PieceOfInformation ;
               rdfs:range :Orientation ;
               rdfs:comment "During an orientation step, no new informatoin is generated but only pre-existing information is recalled" ;
               rdfs:label "was recalled by" .


###  https://w3id.org/tido#wasSelectedBy
:wasSelectedBy rdf:type owl:ObjectProperty ;
               rdfs:domain :Option ;
               rdfs:range :Resolution ;
               rdfs:comment "An option can be selected during a resolution step. This selection of an option is what constitudes a decision." ;
               rdfs:label "was selected by" .


#################################################################
#    Classes
#################################################################

###  http://eturwg.c4i.gmu.edu/files/ontologies/URREF_v5_dev.owl#Information
<http://eturwg.c4i.gmu.edu/files/ontologies/URREF_v5_dev.owl#Information> rdf:type owl:Class ;
                                                                          rdfs:label "Information" .


###  http://www.w3.org/ns/prov#Activity
<http://www.w3.org/ns/prov#Activity> rdf:type owl:Class ;
                                     rdfs:label "Activity" .


###  http://www.w3.org/ns/prov#Agent
<http://www.w3.org/ns/prov#Agent> rdf:type owl:Class ;
                                  rdfs:label "Agent" .


###  http://www.w3.org/ns/prov#Collection
<http://www.w3.org/ns/prov#Collection> rdf:type owl:Class ;
                                       rdfs:label "Collection" .


###  http://www.w3.org/ns/prov#Entity
<http://www.w3.org/ns/prov#Entity> rdf:type owl:Class ;
                                   rdfs:label "Entity" .


###  https://w3id.org/tido#Activity
:Activity rdf:type owl:Class ;
          rdfs:subClassOf <http://www.w3.org/ns/prov#Activity> ,
                          [ rdf:type owl:Restriction ;
                            owl:onProperty :contributesTo ;
                            owl:minQualifiedCardinality "1"^^xsd:nonNegativeInteger ;
                            owl:onClass :Case
                          ] ;
          rdfs:comment "The tido:Activity class is directly inherited from PROV-O. Here, an activity is defined as something that occurs over a period of time and acts upon or with pieces of information; it may include consuming, processing, transforming, modifying, relocating, using, or generating pieces of information." ;
          rdfs:isDefinedBy "https://www.w3.org/TR/2013/REC-prov-o-20130430/#Action" ;
          rdfs:label "Activity" .


###  https://w3id.org/tido#Agent
:Agent rdf:type owl:Class ;
       rdfs:subClassOf <http://www.w3.org/ns/prov#Agent> ;
       rdfs:comment "The tido:Agent class is directly inherited from PROV-O. Here, an agent is defined as something that bears some form of responsibility for an activity taking place, for the existence of an entity, or for another agent's activity" ;
       rdfs:isDefinedBy "https://www.w3.org/TR/2013/REC-prov-o-20130430/#Agent" ;
       rdfs:label "Agent" .


###  https://w3id.org/tido#Case
:Case rdf:type owl:Class ;
      rdfs:subClassOf <http://www.w3.org/ns/prov#Collection> ,
                      [ rdf:type owl:Restriction ;
                        owl:onProperty :investigates ;
                        owl:minQualifiedCardinality "1"^^xsd:nonNegativeInteger ;
                        owl:onClass :RQ
                      ] ;
      rdfs:comment "A collection of pieces of information that were recalled, inferred, deduced or produced during an investigation. " ;
      rdfs:label "Case" ;
      <http://www.w3.org/2004/02/skos/core#altLabel> "Investigation" .


###  https://w3id.org/tido#Consideration
:Consideration rdf:type owl:Class ;
               rdfs:subClassOf :PieceOfInformation ,
                               [ rdf:type owl:Restriction ;
                                 owl:onProperty <http://www.w3.org/ns/prov#wasGeneratedBy> ;
                                 owl:qualifiedCardinality "1"^^xsd:nonNegativeInteger ;
                                 owl:onClass :Evaluation
                               ] ;
               rdfs:comment "A matter weighed or taken into account when formulating an opinion or plan" ;
               rdfs:isDefinedBy "https://www.merriam-webster.com/dictionary/consideration" ;
               rdfs:label "Consideration" .


###  https://w3id.org/tido#Cost
:Cost rdf:type owl:Class ;
      rdfs:subClassOf :Consideration ;
      rdfs:comment "The outlay or expenditure (as of effort or sacrifice) made to achieve an object" ;
      rdfs:isDefinedBy "https://www.merriam-webster.com/dictionary/cost" ;
      rdfs:label "Cost" .


###  https://w3id.org/tido#Evaluation
:Evaluation rdf:type owl:Class ;
            rdfs:subClassOf :Activity ;
            rdfs:comment "A step in the decision process where opinions, evaluations and analysis are expressed. " ;
            rdfs:isDefinedBy "Bales' 2nd phase of group-decision making" ;
            rdfs:label "Evaluation" ;
            <http://www.w3.org/2004/02/skos/core#altLabel> "Evaluation step" .


###  https://w3id.org/tido#Evidence
:Evidence rdf:type owl:Class ;
          rdfs:subClassOf :PieceOfInformation ;
          owl:disjointWith :Hypothesis ;
          rdfs:comment "A piece of information that is either a testamony, an observation, or a sensory measurement." ;
          rdfs:isDefinedBy "http://eturwg.c4i.gmu.edu/files/ontologies/URREF#SingularEvidence" ;
          rdfs:label "Evidence" .


###  https://w3id.org/tido#Goal
:Goal rdf:type owl:Class ;
      rdfs:subClassOf :Consideration ;
      rdfs:comment "A clearly directed intent or purpose" ;
      rdfs:isDefinedBy "https://www.merriam-webster.com/dictionary/aim" ;
      rdfs:label "Goal" .


###  https://w3id.org/tido#Hypothesis
:Hypothesis rdf:type owl:Class ;
            rdfs:subClassOf :PieceOfInformation ,
                            [ rdf:type owl:Restriction ;
                              owl:onProperty <http://www.w3.org/ns/prov#wasGeneratedBy> ;
                              owl:qualifiedCardinality "1"^^xsd:nonNegativeInteger ;
                              owl:onClass :Evaluation
                            ] ;
            rdfs:comment "A possible interpretation of the availble information that forms the ground for further action. Other pieces of information could be used to either support or dispute a hypothesis." ;
            rdfs:isDefinedBy "https://www.merriam-webster.com/dictionary/hypothesis" ;
            rdfs:label "Hypothesis" .


###  https://w3id.org/tido#Option
:Option rdf:type owl:Class ;
        rdfs:subClassOf :PieceOfInformation ,
                        [ rdf:type owl:Restriction ;
                          owl:onProperty <http://www.w3.org/ns/prov#wasGeneratedBy> ;
                          owl:qualifiedCardinality "1"^^xsd:nonNegativeInteger ;
                          owl:onClass :Evaluation
                        ] ;
        rdfs:comment "Something that could be chosen. In the domain of Threat Intelligence, this could mean a course of action, but also an assesment of the situation or the answer to a research question." ;
        rdfs:isDefinedBy "https://www.merriam-webster.com/dictionary/option" ;
        rdfs:label "Option" .


###  https://w3id.org/tido#Orientation
:Orientation rdf:type owl:Class ;
             rdfs:subClassOf :Activity ;
             rdfs:comment "A step in the decision process where available information is shared, repeated, clarified or confirmed." ;
             rdfs:isDefinedBy "Bales' 1st phase of group-decision making" ;
             rdfs:label "Orientation" ;
             <http://www.w3.org/2004/02/skos/core#altLabel> "Orientation step" .


###  https://w3id.org/tido#PieceOfInformation
:PieceOfInformation rdf:type owl:Class ;
                    rdfs:subClassOf <http://eturwg.c4i.gmu.edu/files/ontologies/URREF_v5_dev.owl#Information> ,
                                    <http://www.w3.org/ns/prov#Entity> ,
                                    [ rdf:type owl:Restriction ;
                                      owl:onProperty <http://www.w3.org/ns/prov#wasMemberOf> ;
                                      owl:minQualifiedCardinality "1"^^xsd:nonNegativeInteger ;
                                      owl:onClass :Case
                                    ] ;
                    rdfs:comment "The term “piece of information” is used in this paper in its most general meaning covering other notions such as evidence, knowledge and/or data. A piece of information can be as simple as a measurement (on the scale of real numbers) but could be a fact (i.e., an observation, known to be true), an uncertain statement already modeled into a given mathematical formalism (i.e., a probability distribution), an unstructured statement in natural language" ;
                    rdfs:isDefinedBy "URREF (Costa et al. 2018)" ;
                    rdfs:label "Piece Of Information" ;
                    <http://www.w3.org/2004/02/skos/core#altLabel> "Piece of information" ,
                                                                   "PoI" ,
                                                                   "Sentence" .


###  https://w3id.org/tido#RQ
:RQ rdf:type owl:Class ;
    rdfs:subClassOf :PieceOfInformation ,
                    [ rdf:type owl:Restriction ;
                      owl:onProperty <http://www.w3.org/ns/prov#wasGeneratedBy> ;
                      owl:qualifiedCardinality "1"^^xsd:nonNegativeInteger ;
                      owl:onClass :Evaluation
                    ] ;
    rdfs:comment "A question that arrises during an investigation." ;
    rdfs:label "R Q" ;
    <http://www.w3.org/2004/02/skos/core#altLabel> "RQ" ,
                                                   "Research question" .


###  https://w3id.org/tido#Resolution
:Resolution rdf:type owl:Class ;
            rdfs:subClassOf :Activity ;
            rdfs:comment "A step in the decision process where a possible direction is chosen" ;
            rdfs:isDefinedBy "Bales' 3rd phase of group decision making" ;
            rdfs:label "Resolution" ;
            <http://www.w3.org/2004/02/skos/core#altLabel> "Resolution step" .


###  Generated by the OWL API (version 5.1.18) https://github.com/owlcs/owlapi/
