<?xml version="1.0"?>
<rdf:RDF xmlns="https://w3id.org/tido#"
     xml:base="https://w3id.org/tido"
     xmlns:mod="https://w3id.org/mod#"
     xmlns:owl="http://www.w3.org/2002/07/owl#"
     xmlns:rdf="http://www.w3.org/1999/02/22-rdf-syntax-ns#"
     xmlns:xml="http://www.w3.org/XML/1998/namespace"
     xmlns:xsd="http://www.w3.org/2001/XMLSchema#"
     xmlns:rdfs="http://www.w3.org/2000/01/rdf-schema#"
     xmlns:skos="http://www.w3.org/2004/02/skos/core#"
     xmlns:vann="http://purl.org/vocab/vann/"
     xmlns:terms="http://purl.org/dc/terms/">
    <owl:Ontology rdf:about="https://w3id.org/tido#">
        <owl:versionIRI rdf:resource="https://w3id.org/tido/1.0.0"/>
        <terms:created rdf:datatype="http://www.w3.org/2001/XMLSchema#date">2025-05-07</terms:created>
        <terms:description xml:lang="en">The TIDO ontology can be used to describe the decision processes within the threat intelligence domain</terms:description>
        <terms:license rdf:resource="https://creativecommons.org/licenses/by/4.0/"/>
        <terms:title xml:lang="en">The Threat Intelligence Decision Ontology</terms:title>
        <vann:preferredNamespacePrefix>tido</vann:preferredNamespacePrefix>
        <vann:preferredNamespaceUri rdf:resource="https://w3id.org/tido#"/>
        <owl:versionInfo>1.0.0</owl:versionInfo>
        <mod:createdWith rdf:resource="https://chowlk.linkeddata.es/"/>
    </owl:Ontology>
    


    <!-- 
    ///////////////////////////////////////////////////////////////////////////////////////
    //
    // Annotation properties
    //
    ///////////////////////////////////////////////////////////////////////////////////////
     -->


    


    <!-- http://purl.org/dc/terms/created -->


    <owl:AnnotationProperty rdf:about="http://purl.org/dc/terms/created"/>
    


    <!-- http://purl.org/dc/terms/description -->


    <owl:AnnotationProperty rdf:about="http://purl.org/dc/terms/description"/>
    


    <!-- http://purl.org/dc/terms/license -->


    <owl:AnnotationProperty rdf:about="http://purl.org/dc/terms/license"/>
    


    <!-- http://purl.org/dc/terms/title -->


    <owl:AnnotationProperty rdf:about="http://purl.org/dc/terms/title"/>
    


    <!-- http://purl.org/vocab/vann/preferredNamespacePrefix -->


    <owl:AnnotationProperty rdf:about="http://purl.org/vocab/vann/preferredNamespacePrefix"/>
    


    <!-- http://purl.org/vocab/vann/preferredNamespaceUri -->


    <owl:AnnotationProperty rdf:about="http://purl.org/vocab/vann/preferredNamespaceUri"/>
    


    <!-- http://www.w3.org/2002/07/owl#versionIRI -->


    <owl:AnnotationProperty rdf:about="http://www.w3.org/2002/07/owl#versionIRI"/>
    


    <!-- http://www.w3.org/2002/07/owl#versionInfo -->


    <owl:AnnotationProperty rdf:about="http://www.w3.org/2002/07/owl#versionInfo"/>
    


    <!-- http://www.w3.org/2004/02/skos/core#altLabel -->


    <owl:AnnotationProperty rdf:about="http://www.w3.org/2004/02/skos/core#altLabel"/>
    


    <!-- https://w3id.org/mod#createdWith -->


    <owl:AnnotationProperty rdf:about="https://w3id.org/mod#createdWith"/>
    


    <!-- 
    ///////////////////////////////////////////////////////////////////////////////////////
    //
    // Datatypes
    //
    ///////////////////////////////////////////////////////////////////////////////////////
     -->


    


    <!-- http://www.w3.org/2001/XMLSchema#date -->


    <rdfs:Datatype rdf:about="http://www.w3.org/2001/XMLSchema#date"/>
    


    <!-- 
    ///////////////////////////////////////////////////////////////////////////////////////
    //
    // Object Properties
    //
    ///////////////////////////////////////////////////////////////////////////////////////
     -->


    


    <!-- http://www.w3.org/ns/prov#wasGeneratedBy -->


    <owl:ObjectProperty rdf:about="http://www.w3.org/ns/prov#wasGeneratedBy">
        <rdfs:label>was generated by</rdfs:label>
    </owl:ObjectProperty>
    


    <!-- http://www.w3.org/ns/prov#wasMemberOf -->


    <owl:ObjectProperty rdf:about="http://www.w3.org/ns/prov#wasMemberOf">
        <rdfs:label>was member of</rdfs:label>
    </owl:ObjectProperty>
    


    <!-- https://w3id.org/tido#answers -->


    <owl:ObjectProperty rdf:about="https://w3id.org/tido#answers">
        <rdfs:domain rdf:resource="https://w3id.org/tido#PieceOfInformation"/>
        <rdfs:range rdf:resource="https://w3id.org/tido#RQ"/>
        <rdfs:comment>A piece of information can be used to answer a research question. This piece of information can be anything, as long as it can be expressed in a sentence</rdfs:comment>
        <rdfs:label>answers</rdfs:label>
    </owl:ObjectProperty>
    


    <!-- https://w3id.org/tido#assumes -->


    <owl:ObjectProperty rdf:about="https://w3id.org/tido#assumes">
        <rdfs:domain rdf:resource="https://w3id.org/tido#Option"/>
        <rdfs:range rdf:resource="https://w3id.org/tido#Hypothesis"/>
        <rdfs:comment>A relationship indicating how an option would take an hypothesis as granted or true</rdfs:comment>
        <rdfs:label>assumes</rdfs:label>
        <rdfs:seeAlso>https://www.merriam-webster.com/dictionary/assume</rdfs:seeAlso>
    </owl:ObjectProperty>
    


    <!-- https://w3id.org/tido#contributesTo -->


    <owl:ObjectProperty rdf:about="https://w3id.org/tido#contributesTo">
        <rdfs:domain rdf:resource="https://w3id.org/tido#Activity"/>
        <rdfs:range rdf:resource="https://w3id.org/tido#Case"/>
        <rdfs:label>contributes to</rdfs:label>
    </owl:ObjectProperty>
    


    <!-- https://w3id.org/tido#disputes -->


    <owl:ObjectProperty rdf:about="https://w3id.org/tido#disputes">
        <rdfs:subPropertyOf rdf:resource="https://w3id.org/tido#providesInsightsInto"/>
        <rdfs:domain rdf:resource="https://w3id.org/tido#PieceOfInformation"/>
        <rdfs:range rdf:resource="https://w3id.org/tido#Hypothesis"/>
        <rdfs:comment>A relationship indicating how a piece of information calls into question or casts doubt upon a hypothesis</rdfs:comment>
        <rdfs:label>disputes</rdfs:label>
        <rdfs:seeAlso>https://www.merriam-webster.com/dictionary/dispute</rdfs:seeAlso>
    </owl:ObjectProperty>
    


    <!-- https://w3id.org/tido#hasConsideration -->


    <owl:ObjectProperty rdf:about="https://w3id.org/tido#hasConsideration">
        <rdfs:domain rdf:resource="https://w3id.org/tido#Option"/>
        <rdfs:range rdf:resource="https://w3id.org/tido#Consideration"/>
        <rdfs:comment>An option can have multiple considerations that help in deciding on whether on not to select that option</rdfs:comment>
        <rdfs:label>has consideration</rdfs:label>
    </owl:ObjectProperty>
    


    <!-- https://w3id.org/tido#hasContext -->


    <owl:ObjectProperty rdf:about="https://w3id.org/tido#hasContext">
        <rdfs:domain rdf:resource="https://w3id.org/tido#PieceOfInformation"/>
        <rdfs:range rdf:resource="https://w3id.org/tido#PieceOfInformation"/>
        <rdfs:comment>A relationship indicating how one piece of information provides relevant context to another piece of information.</rdfs:comment>
        <rdfs:label>has context</rdfs:label>
    </owl:ObjectProperty>
    


    <!-- https://w3id.org/tido#informs -->


    <owl:ObjectProperty rdf:about="https://w3id.org/tido#informs">
        <rdfs:domain rdf:resource="https://w3id.org/tido#Option"/>
        <rdfs:range rdf:resource="https://w3id.org/tido#RQ"/>
        <rdfs:comment>A relationship that indicates which options would aid answering a research question. </rdfs:comment>
        <rdfs:label>informs</rdfs:label>
    </owl:ObjectProperty>
    


    <!-- https://w3id.org/tido#investigates -->


    <owl:ObjectProperty rdf:about="https://w3id.org/tido#investigates">
        <rdfs:domain rdf:resource="https://w3id.org/tido#Case"/>
        <rdfs:range rdf:resource="https://w3id.org/tido#RQ"/>
        <rdfs:comment>An investigation, or case, investigates one or more research questions</rdfs:comment>
        <rdfs:label>investigates</rdfs:label>
    </owl:ObjectProperty>
    


    <!-- https://w3id.org/tido#providesInsightsInto -->


    <owl:ObjectProperty rdf:about="https://w3id.org/tido#providesInsightsInto">
        <rdfs:domain rdf:resource="https://w3id.org/tido#PieceOfInformation"/>
        <rdfs:range rdf:resource="https://w3id.org/tido#Hypothesis"/>
        <rdfs:comment>The super-property of tido:supports and tido:disputes</rdfs:comment>
        <rdfs:label>provides insights into</rdfs:label>
        <skos:altLabel>provides insight into</skos:altLabel>
    </owl:ObjectProperty>
    


    <!-- https://w3id.org/tido#questions -->


    <owl:ObjectProperty rdf:about="https://w3id.org/tido#questions">
        <rdfs:domain rdf:resource="https://w3id.org/tido#RQ"/>
        <rdfs:range rdf:resource="https://w3id.org/tido#PieceOfInformation"/>
        <rdfs:comment>A research question can be raised by a piece of information</rdfs:comment>
        <rdfs:label>questions</rdfs:label>
    </owl:ObjectProperty>
    


    <!-- https://w3id.org/tido#supports -->


    <owl:ObjectProperty rdf:about="https://w3id.org/tido#supports">
        <rdfs:subPropertyOf rdf:resource="https://w3id.org/tido#providesInsightsInto"/>
        <rdfs:domain rdf:resource="https://w3id.org/tido#PieceOfInformation"/>
        <rdfs:range rdf:resource="https://w3id.org/tido#Hypothesis"/>
        <rdfs:comment>A relationship indicating how a piece of information provides a hypothesis with substantiation/to support with evidence or authority, making it more certain</rdfs:comment>
        <rdfs:label>supports</rdfs:label>
        <rdfs:seeAlso>https://www.merriam-webster.com/dictionary/supports and https://www.merriam-webster.com/dictionary/corroborate</rdfs:seeAlso>
    </owl:ObjectProperty>
    


    <!-- https://w3id.org/tido#wasExecutedBy -->


    <owl:ObjectProperty rdf:about="https://w3id.org/tido#wasExecutedBy">
        <rdfs:domain rdf:resource="https://w3id.org/tido#Option"/>
        <rdfs:range rdf:resource="https://w3id.org/tido#Activity"/>
        <rdfs:comment>Once an option is selected, it could be excecuted by an activity. </rdfs:comment>
        <rdfs:label>was executed by</rdfs:label>
    </owl:ObjectProperty>
    


    <!-- https://w3id.org/tido#wasRecalledBy -->


    <owl:ObjectProperty rdf:about="https://w3id.org/tido#wasRecalledBy">
        <rdfs:domain rdf:resource="https://w3id.org/tido#PieceOfInformation"/>
        <rdfs:range rdf:resource="https://w3id.org/tido#Orientation"/>
        <rdfs:comment>During an orientation step, no new informatoin is generated but only pre-existing information is recalled</rdfs:comment>
        <rdfs:label>was recalled by</rdfs:label>
    </owl:ObjectProperty>
    


    <!-- https://w3id.org/tido#wasSelectedBy -->


    <owl:ObjectProperty rdf:about="https://w3id.org/tido#wasSelectedBy">
        <rdfs:domain rdf:resource="https://w3id.org/tido#Option"/>
        <rdfs:range rdf:resource="https://w3id.org/tido#Resolution"/>
        <rdfs:comment>An option can be selected during a resolution step. This selection of an option is what constitudes a decision.</rdfs:comment>
        <rdfs:label>was selected by</rdfs:label>
    </owl:ObjectProperty>
    


    <!-- 
    ///////////////////////////////////////////////////////////////////////////////////////
    //
    // Classes
    //
    ///////////////////////////////////////////////////////////////////////////////////////
     -->


    


    <!-- http://eturwg.c4i.gmu.edu/files/ontologies/URREF_v5_dev.owl#Information -->


    <owl:Class rdf:about="http://eturwg.c4i.gmu.edu/files/ontologies/URREF_v5_dev.owl#Information">
        <rdfs:label>Information</rdfs:label>
    </owl:Class>
    


    <!-- http://www.w3.org/ns/prov#Activity -->


    <owl:Class rdf:about="http://www.w3.org/ns/prov#Activity">
        <rdfs:label>Activity</rdfs:label>
    </owl:Class>
    


    <!-- http://www.w3.org/ns/prov#Agent -->


    <owl:Class rdf:about="http://www.w3.org/ns/prov#Agent">
        <rdfs:label>Agent</rdfs:label>
    </owl:Class>
    


    <!-- http://www.w3.org/ns/prov#Collection -->


    <owl:Class rdf:about="http://www.w3.org/ns/prov#Collection">
        <rdfs:label>Collection</rdfs:label>
    </owl:Class>
    


    <!-- http://www.w3.org/ns/prov#Entity -->


    <owl:Class rdf:about="http://www.w3.org/ns/prov#Entity">
        <rdfs:label>Entity</rdfs:label>
    </owl:Class>
    


    <!-- https://w3id.org/tido#Activity -->


    <owl:Class rdf:about="https://w3id.org/tido#Activity">
        <rdfs:subClassOf rdf:resource="http://www.w3.org/ns/prov#Activity"/>
        <rdfs:comment>The tido:Activity class is directly inherited from PROV-O. Here, an activity is defined as something that occurs over a period of time and acts upon or with pieces of information; it may include consuming, processing, transforming, modifying, relocating, using, or generating pieces of information.</rdfs:comment>
        <rdfs:isDefinedBy>https://www.w3.org/TR/2013/REC-prov-o-20130430/#Action</rdfs:isDefinedBy>
        <rdfs:label>Activity</rdfs:label>
    </owl:Class>
    


    <!-- https://w3id.org/tido#Agent -->


    <owl:Class rdf:about="https://w3id.org/tido#Agent">
        <rdfs:subClassOf rdf:resource="http://www.w3.org/ns/prov#Agent"/>
        <rdfs:comment>The tido:Agent class is directly inherited from PROV-O. Here, an agent is defined as something that bears some form of responsibility for an activity taking place, for the existence of an entity, or for another agent&apos;s activity</rdfs:comment>
        <rdfs:isDefinedBy>https://www.w3.org/TR/2013/REC-prov-o-20130430/#Agent</rdfs:isDefinedBy>
        <rdfs:label>Agent</rdfs:label>
    </owl:Class>
    


    <!-- https://w3id.org/tido#Case -->


    <owl:Class rdf:about="https://w3id.org/tido#Case">
        <rdfs:subClassOf rdf:resource="http://www.w3.org/ns/prov#Collection"/>
        <rdfs:subClassOf>
            <owl:Restriction>
                <owl:onProperty rdf:resource="https://w3id.org/tido#investigates"/>
                <owl:minCardinality rdf:datatype="http://www.w3.org/2001/XMLSchema#nonNegativeInteger">1</owl:minCardinality>
            </owl:Restriction>
        </rdfs:subClassOf>
        <rdfs:comment>A collection of pieces of information that were recalled, inferred, deduced or produced during an investigation. </rdfs:comment>
        <rdfs:label>Case</rdfs:label>
        <skos:altLabel>Investigation</skos:altLabel>
    </owl:Class>
    


    <!-- https://w3id.org/tido#Consideration -->


    <owl:Class rdf:about="https://w3id.org/tido#Consideration">
        <rdfs:subClassOf rdf:resource="https://w3id.org/tido#PieceOfInformation"/>
        <rdfs:subClassOf>
            <owl:Restriction>
                <owl:onProperty rdf:resource="http://www.w3.org/ns/prov#wasGeneratedBy"/>
                <owl:allValuesFrom rdf:resource="https://w3id.org/tido#Evaluation"/>
            </owl:Restriction>
        </rdfs:subClassOf>
        <rdfs:comment>A matter weighed or taken into account when formulating an opinion or plan</rdfs:comment>
        <rdfs:isDefinedBy>https://www.merriam-webster.com/dictionary/consideration</rdfs:isDefinedBy>
        <rdfs:label>Consideration</rdfs:label>
    </owl:Class>
    


    <!-- https://w3id.org/tido#Cost -->


    <owl:Class rdf:about="https://w3id.org/tido#Cost">
        <rdfs:subClassOf rdf:resource="https://w3id.org/tido#Consideration"/>
        <rdfs:comment>The outlay or expenditure (as of effort or sacrifice) made to achieve an object</rdfs:comment>
        <rdfs:isDefinedBy>https://www.merriam-webster.com/dictionary/cost</rdfs:isDefinedBy>
        <rdfs:label>Cost</rdfs:label>
    </owl:Class>
    


    <!-- https://w3id.org/tido#Evaluation -->


    <owl:Class rdf:about="https://w3id.org/tido#Evaluation">
        <rdfs:subClassOf rdf:resource="https://w3id.org/tido#Activity"/>
        <rdfs:comment>A step in the decision process where opinions, evaluations and analysis are expressed. </rdfs:comment>
        <rdfs:isDefinedBy>Bales&apos; 2nd phase of group-decision making</rdfs:isDefinedBy>
        <rdfs:label>Evaluation</rdfs:label>
        <skos:altLabel>Evaluation step</skos:altLabel>
    </owl:Class>
    


    <!-- https://w3id.org/tido#Evidence -->


    <owl:Class rdf:about="https://w3id.org/tido#Evidence">
        <rdfs:subClassOf rdf:resource="https://w3id.org/tido#PieceOfInformation"/>
        <owl:disjointWith rdf:resource="https://w3id.org/tido#Hypothesis"/>
        <rdfs:comment>A piece of information that is either a testamony, an observation, or a sensory measurement.</rdfs:comment>
        <rdfs:isDefinedBy>http://eturwg.c4i.gmu.edu/files/ontologies/URREF#SingularEvidence</rdfs:isDefinedBy>
        <rdfs:label>Evidence</rdfs:label>
    </owl:Class>
    


    <!-- https://w3id.org/tido#Goal -->


    <owl:Class rdf:about="https://w3id.org/tido#Goal">
        <rdfs:subClassOf rdf:resource="https://w3id.org/tido#Consideration"/>
        <rdfs:comment>A clearly directed intent or purpose</rdfs:comment>
        <rdfs:isDefinedBy>https://www.merriam-webster.com/dictionary/aim</rdfs:isDefinedBy>
        <rdfs:label>Goal</rdfs:label>
    </owl:Class>
    


    <!-- https://w3id.org/tido#Hypothesis -->


    <owl:Class rdf:about="https://w3id.org/tido#Hypothesis">
        <rdfs:subClassOf rdf:resource="https://w3id.org/tido#PieceOfInformation"/>
        <rdfs:subClassOf>
            <owl:Restriction>
                <owl:onProperty rdf:resource="http://www.w3.org/ns/prov#wasGeneratedBy"/>
                <owl:allValuesFrom rdf:resource="https://w3id.org/tido#Evaluation"/>
            </owl:Restriction>
        </rdfs:subClassOf>
        <rdfs:comment>A possible interpretation of the availble information that forms the ground for further action. Other pieces of information could be used to either support or dispute a hypothesis.</rdfs:comment>
        <rdfs:isDefinedBy>https://www.merriam-webster.com/dictionary/hypothesis</rdfs:isDefinedBy>
        <rdfs:label>Hypothesis</rdfs:label>
    </owl:Class>
    


    <!-- https://w3id.org/tido#Option -->


    <owl:Class rdf:about="https://w3id.org/tido#Option">
        <rdfs:subClassOf rdf:resource="https://w3id.org/tido#PieceOfInformation"/>
        <rdfs:subClassOf>
            <owl:Restriction>
                <owl:onProperty rdf:resource="http://www.w3.org/ns/prov#wasGeneratedBy"/>
                <owl:allValuesFrom rdf:resource="https://w3id.org/tido#Evaluation"/>
            </owl:Restriction>
        </rdfs:subClassOf>
        <rdfs:comment>Something that could be chosen. In the domain of Threat Intelligence, this could mean a course of action, but also an assesment of the situation or the answer to a research question.</rdfs:comment>
        <rdfs:isDefinedBy>https://www.merriam-webster.com/dictionary/option</rdfs:isDefinedBy>
        <rdfs:label>Option</rdfs:label>
    </owl:Class>
    


    <!-- https://w3id.org/tido#Orientation -->


    <owl:Class rdf:about="https://w3id.org/tido#Orientation">
        <rdfs:subClassOf rdf:resource="https://w3id.org/tido#Activity"/>
        <rdfs:comment>A step in the decision process where available information is shared, repeated, clarified or confirmed.</rdfs:comment>
        <rdfs:isDefinedBy>Bales&apos; 1st phase of group-decision making</rdfs:isDefinedBy>
        <rdfs:label>Orientation</rdfs:label>
        <skos:altLabel>Orientation step</skos:altLabel>
    </owl:Class>
    


    <!-- https://w3id.org/tido#PieceOfInformation -->


    <owl:Class rdf:about="https://w3id.org/tido#PieceOfInformation">
        <rdfs:subClassOf rdf:resource="http://eturwg.c4i.gmu.edu/files/ontologies/URREF_v5_dev.owl#Information"/>
        <rdfs:subClassOf rdf:resource="http://www.w3.org/ns/prov#Entity"/>
        <rdfs:subClassOf>
            <owl:Restriction>
                <owl:onProperty rdf:resource="http://www.w3.org/ns/prov#wasMemberOf"/>
                <owl:someValuesFrom rdf:resource="https://w3id.org/tido#Case"/>
            </owl:Restriction>
        </rdfs:subClassOf>
        <rdfs:subClassOf>
            <owl:Restriction>
                <owl:onProperty rdf:resource="http://www.w3.org/ns/prov#wasMemberOf"/>
                <owl:minCardinality rdf:datatype="http://www.w3.org/2001/XMLSchema#nonNegativeInteger">1</owl:minCardinality>
            </owl:Restriction>
        </rdfs:subClassOf>
        <rdfs:comment>The term “piece of information” is used in this paper in its most general meaning covering other notions such as evidence, knowledge and/or data. A piece of information can be as simple as a measurement (on the scale of real numbers) but could be a fact (i.e., an observation, known to be true), an uncertain statement already modeled into a given mathematical formalism (i.e., a probability distribution), an unstructured statement in natural language</rdfs:comment>
        <rdfs:isDefinedBy>URREF (Costa et al. 2018)</rdfs:isDefinedBy>
        <rdfs:label>Piece Of Information</rdfs:label>
        <skos:altLabel>Piece of information</skos:altLabel>
        <skos:altLabel>PoI</skos:altLabel>
        <skos:altLabel>Sentence</skos:altLabel>
    </owl:Class>
    


    <!-- https://w3id.org/tido#RQ -->


    <owl:Class rdf:about="https://w3id.org/tido#RQ">
        <rdfs:subClassOf rdf:resource="https://w3id.org/tido#PieceOfInformation"/>
        <rdfs:subClassOf>
            <owl:Restriction>
                <owl:onProperty rdf:resource="http://www.w3.org/ns/prov#wasGeneratedBy"/>
                <owl:allValuesFrom rdf:resource="https://w3id.org/tido#Evaluation"/>
            </owl:Restriction>
        </rdfs:subClassOf>
        <rdfs:comment>A question that arrises during an investigation.</rdfs:comment>
        <rdfs:label>R Q</rdfs:label>
        <skos:altLabel>RQ</skos:altLabel>
        <skos:altLabel>Research question</skos:altLabel>
    </owl:Class>
    


    <!-- https://w3id.org/tido#Resolution -->


    <owl:Class rdf:about="https://w3id.org/tido#Resolution">
        <rdfs:subClassOf rdf:resource="https://w3id.org/tido#Activity"/>
        <rdfs:comment>A step in the decision process where a possible direction is chosen</rdfs:comment>
        <rdfs:isDefinedBy>Bales&apos; 3rd phase of group decision making</rdfs:isDefinedBy>
        <rdfs:label>Resolution</rdfs:label>
        <skos:altLabel>Resolution step</skos:altLabel>
    </owl:Class>
    


    <!-- 
    ///////////////////////////////////////////////////////////////////////////////////////
    //
    // Annotations
    //
    ///////////////////////////////////////////////////////////////////////////////////////
     -->


    <rdf:Description rdf:about="https://w3id.org/tido#ContributesTo">
        <rdfs:comment>Every activity should contribute to one or more cases/investigations. </rdfs:comment>
        <skos:altLabel>contributes to</skos:altLabel>
    </rdf:Description>
</rdf:RDF>



<!-- Generated by the OWL API (version 5.1.18) https://github.com/owlcs/owlapi/ -->


